

$$a) \vec{E}(r, \theta, t) = E_{\theta} ; \vec{B}(r, \theta, t) = B_{\varphi} ; E_r = E_{\varphi} = B_r = B_{\theta} = 0 \quad (1)$$

$$\begin{aligned} \vec{S}(r, \theta, t) &= \frac{1}{\mu_0} \vec{E}(r, \theta, t) \times \vec{B}(r, \theta, t) = \frac{1}{\mu_0} E_{\theta} B_{\varphi} \hat{\theta} \times \hat{\varphi} = \\ &= -\frac{1}{\mu_0} \left(\frac{\mu_0 \rho_0 \omega^2 \sin \theta}{4\pi} \cos\left(\omega\left(t + \frac{r}{c}\right)\right) \right)^2 \frac{1}{c} \hat{\theta} \times \hat{\varphi} \\ &= -\frac{1}{\mu_0} \frac{\mu_0^2 \rho_0^2 \omega^4 \sin^2 \theta}{16\pi^2} \cos^2\left(\omega\left(t + \frac{r}{c}\right)\right) \frac{1}{c} \hat{r} \quad \hat{\theta} \times \hat{\varphi} = -\hat{r} \\ &= \frac{\mu_0}{c} \frac{\rho_0^2 \omega^4}{16\pi^2} \frac{\sin^2 \theta}{r^2} \cos^2\left(\omega\left(t + \frac{r}{c}\right)\right) \hat{r} \end{aligned}$$

$$b) \langle \vec{S}(r, \theta, t) \rangle = \frac{1}{2} \frac{\mu_0}{c} \frac{\rho_0^2 \omega^4}{16\pi^2} \frac{\sin^2 \theta}{r^2} = \frac{\mu_0}{c} \frac{\rho_0^2 \omega^4}{32\pi^2} \frac{\sin^2 \theta}{r^2}$$

$$\begin{aligned} c) P_z &= \frac{\mu_0}{c} \frac{\rho_0^2 \omega^4}{32\pi^2} \int_{\theta=0}^{\pi} \frac{\sin^2 \theta}{r^2} r^2 \sin \theta d\theta \int_{\varphi=0}^{2\pi} d\varphi \\ &= \frac{\mu_0}{c} \frac{\rho_0^2 \omega^4}{32\pi^2} \int_{\theta=0}^{\pi} \sin^3 \theta d\theta \left[\varphi \right]_0^{2\pi} \\ &= \frac{\mu_0}{c} \rho_0^2 \omega^4 \frac{2\pi}{32\pi^2} \left[\left(\frac{\cos 3\theta}{12} - \frac{3}{4} \cos \theta \right) \right]_0^{\pi} \\ &= \frac{\mu_0}{c} \rho_0^2 \omega^4 \frac{1}{16\pi} \left[\frac{\cos 3\pi}{12} - \frac{3}{4} \cos \pi - \left(\frac{\cos(0)}{12} - \frac{3}{4} \cos(0) \right) \right] \\ &= \frac{\mu_0}{c} \rho_0^2 \omega^4 \frac{1}{16\pi} \left[-\frac{1}{12} - \frac{3}{4}(-1) - \left(\frac{1}{12} - \frac{3}{4} \right) \right] \\ &= \frac{\mu_0}{c} \rho_0^2 \omega^4 \frac{1}{16\pi} \left[-\frac{2}{12} + \frac{6}{4} \right] = \frac{\mu_0}{c} \frac{\rho_0^2 \omega^4}{16\pi} \left[\frac{-2+18}{12} \right] = \frac{\mu_0}{c} \frac{\rho_0^2 \omega^4}{16\pi} \frac{16}{12} = \end{aligned}$$

$$= \frac{\mu_0}{c} \frac{\rho_0^2 \omega^4}{12\pi}$$

(2)

$$d) \mu_0 = \frac{1}{\epsilon_0 c^2} ; \omega = 2\pi\nu ; \nu = \frac{1}{T} ; c = \lambda\nu$$

$$P = \frac{\mu_0}{c} \frac{\rho_0^2 \omega^4}{12\pi} = \frac{1}{\epsilon_0 c^2} \frac{1}{c} \frac{\rho_0^2 (2\pi\nu)^4}{12\pi} = \frac{1}{\epsilon_0} \frac{1}{\lambda^3 \nu^3} \frac{\rho_0^2 (2\pi)^4 \nu^4}{12\pi} =$$

$$= \frac{\rho_0^2 (2\pi)^4 \nu}{\epsilon_0 2\pi 6 \lambda^3 \nu^3} = \frac{\rho_0^2 (2\pi)^3 \nu}{6 \epsilon_0 \lambda^3} = \frac{(2\pi)^3}{6} \frac{\rho_0^2}{\epsilon_0} \frac{1}{\lambda^3 c}$$

$$e) [P] = \frac{C \cancel{m^2}}{\cancel{s}} V \cancel{m} \frac{1}{\cancel{s}} = \frac{CV}{s} = \frac{J}{s} = \text{Watt}$$

Linac - Bremsstrahlung

Jet radio synchrotron